Notice that
\begin{align*}
    k(x,y)
    &= \exp\left(\frac{-\|x-y\|^2}{2\sigma^2}\right)\\
    &= \exp\left(\frac{-(\|x\|^2 - 2\ipt{x,y} + \|y\|^2)}{2\sigma^2}\right)\\
    &= \exp\left(\frac{-\|x\|^2}{2\sigma^2}\right)
    \exp\left(\frac{-\|y\|^2}{2\sigma^2}\right)
    \exp\left(\frac{\ipt{x,y}}{\sigma^2}\right).
\end{align*}
Let \(g(x) = \exp\left(-\|x\|^2/2\sigma^2\right)\), \(k_1(x,y) = g(x)g(y)\), and \(k_2(x,y) = \ipt{x,y}/\sigma^2\).
By \cref{itm:constructing-kernels-5}, \(k_1\) is a kernel.
Since \(\ipt{x,y}\) is a kernel and \(1/\sigma^2 >0\), \cref{itm:constructing-kernels-1} implies \(k_2\) is a kernel and \cref{itm:constructing-kernels-6} implies \(\exp(k_2(x,y))\) is a kernel.
Therefore, by \cref{itm:constructing-kernels-2},
\begin{equation}
    k(x,y) = g(x)g(y) \exp(k_2(x,y)) = k_1(x,y) \exp(k_2(x,y))
\end{equation}
is a kernel.