Suppose \(k_1\) and \(k_2\) are kernels on \(\X \times \X\).
The following functions kernels.
\begin{enumerate}
    \item \label{itm:constructing-kernels-1}
    \(k(x,y) = a_1 k_1(x,y) + a_2 k_2(x,y)\) for all \(a_1, a_2 \geq 0\).
    \item \label{itm:constructing-kernels-2}
    \(k(x,y) = k_1(x,y) k_2(x,y)\).
    \item \label{itm:constructing-kernels-3}
    \(k(x,y) = a_0 + a_1 k_1(x,y) + a_2 k_1(x,y)^2 + \cdots + a_n k_1(x,y)^n\) for all \(n \in \NN\) and \(a_0, \dots, a_n \geq 0\).
    \item \label{itm:constructing-kernels-4}
    \(k(x,y) = k_1(h(x),h(y))\) for all \(h : \X \to \X\).
    \item \label{itm:constructing-kernels-5}
    \(k(x,y) = g(x)g(y)\) for all \(g : \X \to \RR\).
    \item \label{itm:constructing-kernels-6}
    \(k(x,y) = \exp(k_1(x,y))\).
\end{enumerate}